Get category language working

src/EasyWF.v
@@ -9,9 +9,257 @@ Unset Strict Implicit.
 Unset Printing Implicit Defensive.
 Set Bullet Behavior "Strict Subproofs".
 
-(* TODO: change from loads to imports *)
-From excomp Require Import Utils Exp Rule CoreDefs Core.
+From excomp Require Import Utils Exp Rule Core.
 
+
+Import OptionMonad.
+
+Definition nth_level_err {A} l n : option A :=
+  if n < size l then List.nth_error l (size l - n.+1) else None.
+
+Lemma is_nth_level_to_fn_err {A:eqType} (l : seq A) n x
+  : is_nth_level l n x = (nth_level_err l n == Some x).
+Proof using .
+  unfold nth_level_err; unfold is_nth_level.
+  case: (n < size l); simpl; try easy.
+Qed.
+
+(* TODO: differentiate out of fuel? or just calculate enough? or use Function w/ measure? *)
+
+Fixpoint type_wf_term l c e {struct e} : option exp :=
+  (* output context not easily inferred; has to be an argument 
+       inlined to get termination checking working *)
+  let type_wf_subst := fix twfs l c s (c' : ctx) {struct s} : option unit :=
+                         match s, c' with
+                         | [::], [::] => Some tt
+                         | e::s', t::c'' =>
+                           do t' <- type_wf_term l c e;
+                           do tt <- check (t' == t[/s'/]);
+                           twfs l c s' c''
+                         | _,_ => None
+                         end in
+  match e with
+  | con n s =>
+    do term_rule c' t <- nth_level_err l n;
+    do tt <- type_wf_subst l c s c';
+    Some t[/s/]
+  (* TODO: incorporate into other constrs
+         | conv pf e' =>
+           do t <- type_wf_term l c e';
+           do (t1,t2) <- type_le_sort l c pf;
+           do tt <- check (t == t1);
+           ret t2 *)
+  | var n =>
+    do e <- nth_level_err c n;
+    Some e
+  end.
+
+Definition type_wf_subst := fix twfs l c s (c' : ctx) {struct s} : option unit :=
+                              match s, c' with
+                              | [::], [::] => Some tt
+                              | e::s', t::c'' =>
+                                do t' <- type_wf_term l c e;
+                                do tt <- check (t' == t[/s'/]);
+                                twfs l c s' c''
+                              | _,_ => None
+                              end. 
+
+Definition type_wf_sort l c (t : exp) : option unit :=
+  match t with
+  | con n s =>
+    do sort_rule c' <- nth_level_err l n;
+    do tt <- type_wf_subst l c s c';
+    Some tt
+  | var _ => None
+  end.
+
+Lemma option_id_match {A} (me : option A)
+  :  match me with
+     | Some e => Some e
+     | None => None
+     end = me.
+Proof using .
+  by case me.
+Qed.
+
+Ltac break_option_dos :=
+  (* TODO: hack for case:*)
+  let nxtnxtnxt := fresh "nxtnxtnxt" in
+  repeat
+    (match goal with
+       |-context[match ?e with _ => _ end] =>
+       case nxtnxtnxt: e end; try easy;
+     let H := fresh "casevar" in move: nxtnxtnxt => H).
+
+Lemma type_wf_term_recognizes l c e t
+  : wf_ctx l c -> type_wf_term l c e = Some t -> wf_term l c e t.
+Proof with eauto with judgment using .
+  elim: e c t.
+  {
+    simpl; intros until t; intro wfc.
+    rewrite option_id_match; move /eqP; rewrite -is_nth_level_to_fn_err...
+  }
+  {
+    intros until t; intro wfc.
+    simpl.
+    break_option_dos.
+    subst.
+    case => <-. move: casevar => /eqP.
+    rewrite -is_nth_level_to_fn_err.
+    intro isn. apply: wf_term_by'; eauto.
+    move: isn casevar1.
+    match goal with
+      |- _ -> _ -> wf_subst _ _ _ ?c => move: c => c' end.
+    move => isn.
+    suff: wf_ctx l c'.
+    clear isn.
+    elim: l0 H c'; simpl.
+    move => _ c';break_option_dos...
+    {
+      intro_to and; case => IH1 IH2.
+      case; simpl; try easy.
+      intros t' c'.
+      break_option_dos...
+      subst.
+      move: (IH1 c _ wfc casevar) => wft.
+      move: casevar0.
+      unfold check.
+      match goal with |-context[if ?A then _ else _] => case aeq: A end; try easy.
+      move => _.
+      move: aeq wft => /eqP -> wft.
+      intros.
+      inversion x;  subst.
+      apply: wf_subst_cons'...
+    }
+    move: isn.
+    suff: wf_lang l...
+    move => wfl.
+    move /is_nth_level_in /(rule_in_wf wfl).
+    inversion...
+  }
+Qed.    
+
+Lemma type_wf_subst_recognizes l c s c'
+  : wf_ctx l c -> wf_ctx l c' -> type_wf_subst l c s c' = Some tt -> wf_subst l c s c'.
+Proof using .
+  intros wfc.
+  elim: s c'; intros until c'; case: c'; simpl; try easy; eauto with judgment.
+  intros t' c' wfc'.
+  inversion wfc'; subst.
+  break_option_dos...
+  subst.
+  move /(H c' H4) => wfs.
+  apply: wf_subst_cons'; eauto with judgment.
+  move: casevar0.
+  unfold check.
+  match goal with |-context[if ?A then _ else _] => case aeq: A end; try easy.
+  move: aeq casevar => /eqP ->.
+  move / type_wf_term_recognizes.
+  eauto with judgment.
+Qed.
+
+Lemma type_wf_sort_recognizes l c t
+  : wf_ctx l c -> type_wf_sort l c t = Some tt -> wf_sort l c t.
+Proof.
+  case: t; simpl; try easy.
+  intros n s.
+  break_option_dos.
+  subst.
+  move: casevar => /eqP.
+  rewrite - is_nth_level_to_fn_err .
+  move => isn; pose p:= isn; move: p.
+  move /is_nth_level_in /rule_in_wf.
+  intros limplr wfc _.
+  suff: wf_lang l; eauto with judgment.
+  move /limplr; inversion; try easy.
+  subst.
+  move: casevar1 => /type_wf_subst_recognizes.
+  eauto with judgment.
+Qed.
+
+Fixpoint type_wf_ctx l c : option unit :=
+  match c with
+  | [::] => Some tt
+  | t::c' =>
+    do tt <- type_wf_sort l c' t;
+    type_wf_ctx l c'
+  end.
+
+
+Lemma type_wf_ctx_recognizes l c
+  : wf_lang l -> type_wf_ctx l c = Some tt -> wf_ctx l c.
+Proof using .
+  elim: c; simpl; eauto with judgment.
+  intros t c.
+  break_option_dos.
+  subst.
+  move => H /H => H1 /H1.
+  move: casevar => /type_wf_sort_recognizes.
+  eauto with judgment.
+Qed.
+
+Definition type_wf_rule l r : option unit :=
+  match r with
+  | sort_rule c => type_wf_ctx l c
+  | term_rule c t =>
+    do tt <- type_wf_sort l c t;
+    type_wf_ctx l c
+  | sort_le c t1 t2 =>
+    do tt <- type_wf_sort l c t1;
+    do tt <- type_wf_sort l c t2;
+    type_wf_ctx l c
+  | term_le c e1 e2 t =>
+    do t1 <- type_wf_term l c e1;
+    do t2 <- type_wf_term l c e2;
+    do tt <- check (t == t1);
+    do tt <- check (t == t2);
+    type_wf_ctx l c
+  end.
+
+Lemma type_wf_rule_recognizes l r
+  : wf_lang l -> type_wf_rule l r = Some tt -> wf_rule l r.
+Proof using .
+  case: r; simpl; intro_to wf_lang; break_option_dos; intro wfl; subst.
+  all: move /type_wf_ctx_recognizes.
+  eauto with judgment.
+  all: repeat match goal with
+  | H : type_wf_sort _ _ _= Some tt |- _ =>
+    move: H => /type_wf_sort_recognizes
+  end; eauto 7 with judgment.
+
+  move: casevar1 casevar3.
+  repeat match goal with
+           |- context[check ?B] =>
+           case nxt: B; move: nxt; simpl; move /eqP
+         end; try easy.
+  move ->.
+  intro; subst.
+  repeat match goal with
+         | H : type_wf_term _ _ _ = Some _ |- _ =>
+           move: H => /type_wf_term_recognizes
+         end; eauto 7 with judgment.
+Qed.  
+
+Fixpoint type_wf_lang l : option unit :=
+  match l with
+  | [::] => Some tt
+  | r::l' =>
+    do tt <- type_wf_rule l' r;
+    type_wf_lang l'
+  end.
+
+Lemma type_wf_lang_recognizes l
+  : type_wf_lang l = Some tt -> wf_lang l.
+Proof using .
+  elim: l; simpl; eauto with judgment; intros r l; break_option_dos.
+  intros.
+  subst.
+  move: casevar => /type_wf_rule_recognizes.
+  eauto with judgment.
+Qed.
+
+
+  (*
 
 Definition lookup_sort_args l n : option ctx :=
   match nth_level l n with
@@ -449,4 +697,5 @@ Ltac view_with_is_easy_IH :=
   match goal with
   | |- ?E -> _ =>
     let exp_head 
+*)
 *)
